ifc/noninterferenceS.v
@@ -1,0 +1,92 @@
+From mathcomp Require Import
+  ssreflect ssrfun ssrbool ssrnat eqtype seq choice fintype finfun.
+From CoqUtils Require Import hseq ord fset partmap word.
+From MicroPolicies Require Import
+  lib.utils lib.partmap_utils common.types symbolic.symbolic symbolic.exec
+  ifc.labels ifc.common ifc.symbolic ifc.abstract ifc.noninterference ifc.refinementSA.
+
+Set Implicit Arguments.
+Unset Strict Implicit.
+Unset Printing Implicit Defensive.
+
+Section Noninterference.
+
+Import DoNotation.
+
+Variable L : labType.
+Variable mt : machine_types.
+Variable mops : machine_ops mt.
+Variable r_arg1 : reg mt.
+Variable r_arg2 : reg mt.
+Variable r_ret : reg mt.
+Variable output_addr : mword mt.
+Variable call_addr : mword mt.
+Variable return_addr : mword mt.
+
+Local Notation word := (mword mt).
+Local Notation d_atom := (atom word L).
+
+Local Notation sstate := (@Symbolic.state mt (sym_ifc L mt)).
+Local Notation sstep :=
+  (@stepf _ _ _ (@ifc_syscalls L mt mops r_arg1 r_arg2 r_ret
+                               output_addr call_addr return_addr)).
+Local Notation strace :=
+  (@symbolic.trace _ _ _ r_arg1 r_arg2 r_ret
+                   output_addr call_addr return_addr).
+Local Notation astate := (ifc.abstract.state L mt).
+Local Notation astep := (@step L mt mops r_arg1 r_arg2 r_ret
+                               output_addr call_addr return_addr).
+Local Notation atrace :=
+  (@abstract.trace _ _ _
+                   r_arg1 r_arg2 r_ret
+                   output_addr call_addr return_addr).
+Implicit Types (st : sstate).
+
+Local Open Scope label_scope.
+
+Inductive s_indist rs st1 st2 :=
+| SIndist of  taga (Symbolic.pc st1) ⊑ rs
+             &  Symbolic.pc st1 = Symbolic.pc st2
+             &  pointwise (indist taga rs)
+                          (Symbolic.regs st1) (Symbolic.regs st2)
+             &  pointwise (indist (fun t =>
+                                     if taga t is MemData rl
+                                     then rl
+                                     else ⊥) rs)
+                          (Symbolic.mem st1) (Symbolic.mem st2)
+             & Symbolic.internal st1 = IntIFC [::] [::]
+             & Symbolic.internal st2 = IntIFC [::] [::].
+
+Theorem noninterference rs st1 st2 n1 n2 :
+  s_indist rs st1 st2 ->
+  indist_seq_prefix eq
+                    [seq x <- strace n1 st1 | taga x ⊑ rs]
+                    [seq x <- strace n2 st2 | taga x ⊑ rs].
+Proof.
+move=> ind.
+have {ind} ind:
+  noninterference.s_indist rs (abs_of_sym mops st1) (abs_of_sym mops st2).
+  case: ind => lo_pc e_pc ind_r ind_m int01 int02.
+  rewrite /abs_of_sym; apply: SIndistLow=> //=.
+    move=> ptr; rewrite !mapmE /=.
+    move: (ind_m ptr).
+    case: (Symbolic.mem st1 ptr) => [[v1 l1]|] //=;
+    case: (Symbolic.mem st2 ptr) => [[v2 l2]|] //=.
+    rewrite /indist /=.
+    case: l1 l2 => [|l1] [|l2] //=; rewrite ?botP ?orbT ?eqxx /= => /eqP //.
+    by move => [<-].
+  by rewrite int01 int02 /=.
+have [t1 et1] : exists t, atrace n1 (abs_of_sym mops st1) = strace n1 st1 ++ t.
+  exact/refinement/abs_of_symP.
+have [t2 et2] : exists t, atrace n2 (abs_of_sym mops st2) = strace n2 st2 ++ t.
+  exact/refinement/abs_of_symP.
+have:
+  indist_seq_prefix eq
+                    [seq x <- atrace n1 (abs_of_sym mops st1) | taga x ⊑ rs]
+                    [seq x <- atrace n2 (abs_of_sym mops st2) | taga x ⊑ rs].
+  exact: noninterference ind.
+rewrite et1 et2 !filter_cat.
+exact: indist_seq_prefix_sub.
+Qed.
+
+End Noninterference.
